src/Narcissus/Examples/NetworkStack/UDP_Packet.v
@@ -83,6 +83,18 @@ Section UDP_Decoder.
   (* Step Two and a Half: Add some simple facts about correct packets
    for the decoder automation. *)
 
+  Lemma CorrectDecoder_foo s len_format1 len_format2 :
+    CorrectDecoderFor (fun n => n = len_format1 s + len_format2 s + 16) (fun n : nat => UDP_Packet_Format s).
+    unfold UDP_Packet_Format.
+    eapply Start_CorrectDecoderFor.
+    apply_rules.
+
+    start_synthesizing_decoder.
+    econstructor.
+
+
+    (format1 ++ format_unused_word 16 ++ format2)%format decodeA P) ->
+
   Lemma UDP_Packet_Header_Len_OK
     : forall (a : UDP_Packet) (ctx ctx' ctx'' : CacheFormat) (c : word 16) (b b'' ext : ByteString),
       (format_word ◦ SourcePort ++ format_word ◦ DestPort ++ format_nat 16 ◦ Init.Nat.add 8 ∘ (projT1 (P:=ByteBuffer.t) ∘ Payload)) a
@@ -96,6 +108,7 @@ Section UDP_Decoder.
                     (mappend (format_checksum ByteString AlignedByteString.ByteStringQueueMonoid ByteString_QueueMonoidOpt 16 c) b'')) ext).
   Proof.
     intros; simpl.
+    clear H0.
     pose proof mappend_assoc as H''; simpl in H'';
       rewrite <- !H''.
     unfold UDP_Packet_format_measure.
